theories/coneris/examples/hash/con_hash_impl1.v
@@ -3,7 +3,7 @@ From iris.proofmode Require Import proofmode.
 From iris Require Import ghost_map.
 From iris.algebra Require Import excl_auth gmap.
 From clutch.prelude Require Import stdpp_ext.
-From clutch.coneris Require Import coneris hocap_rand lib.map hash_view_interface lock con_hash_interface1.
+From clutch.coneris Require Import coneris hash_view_interface con_hash_interface0 con_hash_interface1.
 
 Set Default Proof Using "Type*".
 
@@ -37,166 +37,149 @@ Set Default Proof Using "Type*".
 
 (* End lemmas. *)
 
-Section lemmas.
-  Context `{!inG Σ (excl_authR (gmapO nat natO))}.
+(* Section lemmas. *)
+(*   Context `{!inG Σ (excl_authR (gmapO nat natO))}. *)
 
-  (* Helpful lemmas *)
-  Lemma ghost_var_alloc b :
-    ⊢ |==> ∃ γ, own γ (●E b) ∗ own γ (◯E b).
-  Proof.
-    iMod (own_alloc (●E b ⋅ ◯E b)) as (γ) "[??]".
-    - by apply excl_auth_valid.
-    - by eauto with iFrame.
-  Qed.
+(*   (* Helpful lemmas *) *)
+(*   Lemma ghost_var_alloc b : *)
+(*     ⊢ |==> ∃ γ, own γ (●E b) ∗ own γ (◯E b). *)
+(*   Proof. *)
+(*     iMod (own_alloc (●E b ⋅ ◯E b)) as (γ) "[??]". *)
+(*     - by apply excl_auth_valid. *)
+(*     - by eauto with iFrame. *)
+(*   Qed. *)
 
-  Lemma ghost_var_agree γ b c :
-    own γ (●E b) -∗ own γ (◯E c) -∗ ⌜ b = c ⌝.
-  Proof.
-    iIntros "Hγ● Hγ◯".
-    by iCombine "Hγ● Hγ◯" gives %->%excl_auth_agree_L.
-  Qed.
+(*   Lemma ghost_var_agree γ b c : *)
+(*     own γ (●E b) -∗ own γ (◯E c) -∗ ⌜ b = c ⌝. *)
+(*   Proof. *)
+(*     iIntros "Hγ● Hγ◯". *)
+(*     by iCombine "Hγ● Hγ◯" gives %->%excl_auth_agree_L. *)
+(*   Qed. *)
 
-  Lemma ghost_var_update γ b' b c :
-    own γ (●E b) -∗ own γ (◯E c) ==∗ own γ (●E b') ∗ own γ (◯E b').
-  Proof.
-    iIntros "Hγ● Hγ◯".
-    iMod (own_update_2 _ _ _ (●E b' ⋅ ◯E b') with "Hγ● Hγ◯") as "[$$]".
-    { by apply excl_auth_update. }
-    done.
-  Qed.
+(*   Lemma ghost_var_update γ b' b c : *)
+(*     own γ (●E b) -∗ own γ (◯E c) ==∗ own γ (●E b') ∗ own γ (◯E b'). *)
+(*   Proof. *)
+(*     iIntros "Hγ● Hγ◯". *)
+(*     iMod (own_update_2 _ _ _ (●E b' ⋅ ◯E b') with "Hγ● Hγ◯") as "[$$]". *)
+(*     { by apply excl_auth_update. } *)
+(*     done. *)
+(*   Qed. *)
 
-End lemmas.
+(* End lemmas. *)
 
 
 Section con_hash_impl1.
+  
+  Variable val_size:nat.
   Context `{Hc: conerisGS Σ, Hs: !ghost_mapG Σ nat (),
               h : @hash_view Σ Hc, Hhv: hvG Σ,
-                lo:lock, Hl: lockG Σ,
-                  r: @rand_spec Σ Hc, Hr: randG Σ,
-                    Hm: inG Σ (excl_authR (gmapO nat natO))}.
-  Variable val_size:nat.
+               hash0: !con_hash0 val_size
+    }.
 
   (** * Code *)
-  Definition init_hash_state : val := init_map.
 
-  Definition compute_hash : val :=
-    λ: "hm" "v" "α",
-      match: get "hm" "v" with
-      | SOME "b" => "b"
-      | NONE =>
-          let: "b" := (rand_tape "α" #val_size) in
-          set "hm" "v" "b";;
-          "b"
-      end.
+  Definition init_hash:=init_hash0.
+  Definition compute_hash:=compute_hash0.
+  Definition allocate_tape:=allocate_tape0.
+
   
-  Definition compute_con_hash :val:=
-    λ: "lhm" "v" "α",
-      let, ("l", "hm") := "lhm" in
-      acquire "l";;
-      let: "output" := compute_hash "hm" "v" "α" in
-      release "l";;
-      "output".
-  
-  (* init_hash returns a hash as a function, basically wrapping the internal state
-     in the returned function *)
-  Definition init_hash : val :=
-    λ: "_",
-      let: "hm" := init_hash_state #() in
-      let: "l" := newlock #() in
-      compute_con_hash ("l", "hm").
-
-  Definition allocate_tape : val :=
-    λ: "_",
-      rand_allocate_tape #val_size.
-
-
-  Definition compute_con_hash_specialized (lhm:val):val:=
-    λ: "v" "α",
-      let, ("l", "hm") := lhm in
-      acquire "l";;
-      let: "output" := (compute_hash "hm") "v" "α" in
-      release "l";;
-      "output".
-
-  Definition set_frag v (γ:gname) :=(v ↪[γ]□ ())%I.
-  
-  Definition hash_tape α t γ :=(rand_tapes (L:=Hr) α (val_size, t)∗ [∗ list] n ∈ t, set_frag n γ)%I.
-  Definition con_hash_view k v γ γ' := (hv_frag (L:=Hhv) k v γ ∗ set_frag v γ')%I.
-  Definition abstract_con_hash (f:val) (l:val) (hm:val) γ1 γ2 γ3: iProp Σ :=
-    ∃ m,
-      ⌜f=compute_con_hash_specialized (l, hm)%V⌝ ∗
-      hv_auth (L:=Hhv) m γ1 ∗
-      own γ2 (●E m) ∗
-      ([∗ map] k↦v∈m, set_frag v γ3) 
-  .
-  Definition abstract_con_hash_inv f l hm γ1 γ2 γ3:=
-    inv (nroot.@"con_hash_abstract") (abstract_con_hash f l hm γ1 γ2 γ3).
-  
-  Definition concrete_con_hash (hm:val) (m:gmap nat nat) γ : iProp Σ:=
-    ∃ (hm':loc), ⌜hm=#hm'⌝ ∗
-    map_list hm' ((λ b, LitV (LitInt (Z.of_nat b))) <$> m) ∗
-    own γ (◯E m).
-
-  Definition concrete_con_hash_inv hm l γ_lock γ:=
-    is_lock (L:=Hl) γ_lock l (∃ m, concrete_con_hash hm m γ).
-  
-  Definition con_hash_inv f l hm γ1 γ3 γ_lock:=
-    (∃ γ2, abstract_con_hash_inv f l hm γ1 γ2 γ3 ∗
-     concrete_con_hash_inv hm l γ_lock γ2)%I.
-
-  Definition hash_set s γ3 := (ghost_map_auth γ3 1 (gset_to_gmap () s) ∗
+  Definition hash_set_frag v (γ:gname) :=(v ↪[γ]□ ())%I.
+  Definition hash_set s γ:=(ghost_map_auth γ 1 (gset_to_gmap () s) ∗
                               ⌜ ∀ x, x∈s-> (x < S val_size)%nat⌝ ∗
-                                     [∗ set] x∈s, set_frag x γ3
-                             )%I
-  .
+                                     [∗ set] x∈s, hash_set_frag x γ
+                             )%I.
+  Definition hash_auth m γ1 γ2:=
+    (hv_auth (L:=Hhv) m γ1 ∗
+     [∗ map] v∈m, hash_set_frag v γ2)%I.
+  Definition hash_tape α ns γ2 γ_tape :=
+    (hash_tape0 α ns γ_tape∗ [∗ list] n ∈ ns, hash_set_frag n γ2)%I.
+  Definition hash_tape_auth m γ_set γ :=
+    (hash_tape_auth0 m γ ∗
+     [∗ map]ns ∈m, [∗ list] x ∈ ns, hash_set_frag x γ_set
+    )%I.
 
-  (** γ1 is hash view 
-      γ2 is map 
-      γ3 is gmap of numbers sampled
-   *)
+  Definition hash_frag k v γ1 γ2:=
+    (hv_frag (L:=Hhv) k v γ1 ∗
+     hash_set_frag v γ2)%I.
+
+  Definition con_hash_inv N f l hm (P:gmap nat nat -> gmap val (list nat) -> iProp Σ) {HP: ∀ m m', Timeless (P m m')} γ1 γ2 γ_lock:=
+    con_hash_inv0 N f l hm (λ m m', hash_auth m γ1 γ2 ∗ ([∗ map]ns ∈m', [∗ list] x ∈ ns, hash_set_frag x γ2) ∗ P m m')%I γ_lock.
+
   
-  Lemma con_hash_view_in_hash_set γ1 γ3 s v res:
-    con_hash_view v res γ1 γ3 -∗ hash_set s γ3 -∗ ⌜res ∈ s⌝.
+  Lemma hash_set_frag_in_set s n γ:
+    hash_set s γ -∗ hash_set_frag n γ -∗ ⌜n ∈ s⌝.
   Proof.
-    iIntros "H1 H2".
-    rewrite /con_hash_view/hash_set/set_frag.
-    iDestruct "H1" as "[_ H1]".
-    iDestruct "H2" as "[H2 _]".
+    iIntros "(H1 &_) H2".
+    rewrite /hash_set/hash_set_frag.
     iCombine "H1 H2" gives "%H".
     iPureIntro.
     rewrite lookup_gset_to_gmap_Some in H. naive_solver.
   Qed.
+  
+  
+  (* Definition hash_tape α t γ :=(rand_tapes (L:=Hr) α (val_size, t)∗ [∗ list] n ∈ t, set_frag n γ)%I. *)
+  (* Definition con_hash_view k v γ γ' := (hv_frag (L:=Hhv) k v γ ∗ set_frag v γ')%I. *)
+  (* Definition abstract_con_hash (f:val) (l:val) (hm:val) γ1 γ2 γ3: iProp Σ := *)
+  (*   ∃ m, *)
+  (*     ⌜f=compute_con_hash_specialized (l, hm)%V⌝ ∗ *)
+  (*     hv_auth (L:=Hhv) m γ1 ∗ *)
+  (*     own γ2 (●E m) ∗ *)
+  (*     ([∗ map] k↦v∈m, set_frag v γ3)  *)
+  (* . *)
+  (* Definition abstract_con_hash_inv f l hm γ1 γ2 γ3:= *)
+  (*   inv (nroot.@"con_hash_abstract") (abstract_con_hash f l hm γ1 γ2 γ3). *)
+  
+  (* Definition concrete_con_hash (hm:val) (m:gmap nat nat) γ : iProp Σ:= *)
+  (*   ∃ (hm':loc), ⌜hm=#hm'⌝ ∗ *)
+  (*   map_list hm' ((λ b, LitV (LitInt (Z.of_nat b))) <$> m) ∗ *)
+  (*   own γ (◯E m). *)
 
-  Lemma tape_in_hash_set α ns γ s:
-    hash_tape α ns γ -∗ hash_set s γ -∗ ⌜Forall (λ x, x∈s) ns⌝.
+  (* Definition concrete_con_hash_inv hm l γ_lock γ:= *)
+  (*   is_lock (L:=Hl) γ_lock l (∃ m, concrete_con_hash hm m γ). *)
+  
+  (* Definition con_hash_inv f l hm γ1 γ3 γ_lock:= *)
+  (*   (∃ γ2, abstract_con_hash_inv f l hm γ1 γ2 γ3 ∗ *)
+  (*    concrete_con_hash_inv hm l γ_lock γ2)%I. *)
+
+  (* Definition hash_set s γ3 := (ghost_map_auth γ3 1 (gset_to_gmap () s) ∗ *)
+  (*                             ⌜ ∀ x, x∈s-> (x < S val_size)%nat⌝ ∗ *)
+  (*                                    [∗ set] x∈s, set_frag x γ3 *)
+  (*                            )%I *)
+  (* . *)
+
+  
+  Lemma hash_frag_in_hash_set γ1 γ3 s v res:
+    hash_frag v res γ1 γ3 -∗ hash_set s γ3 -∗ ⌜res ∈ s⌝.
   Proof.
-    iIntros "[_ #H1] [H2 _]".
+    iIntros "[_ #H1] H2".
+    iApply (hash_set_frag_in_set with "[$][$]").
+  Qed.
+
+  Lemma tape_in_hash_set α ns γ γ_tape s:
+    hash_tape α ns γ γ_tape -∗ hash_set s γ -∗ ⌜Forall (λ x, x∈s) ns⌝.
+  Proof.
+    iIntros "[_ #H1] H2".
     rewrite Forall_forall.
     iIntros (x Hx).
     iDestruct (big_sepL_elem_of with "[$]") as "H"; first done.
-    iCombine "H2 H" gives "%".
-    iPureIntro.
-    rewrite lookup_gset_to_gmap_Some in H. naive_solver.
+    iApply (hash_set_frag_in_set with "[$][$]").
   Qed.
 
-  Lemma con_hash_presample γ3 E (ε εI εO:nonnegreal) ns α s :
+  Lemma hash_tape_presample m γ γ_set α ns s (ε εI εO:nonnegreal) E:
     (εI * (size s) + εO * (val_size + 1 - size s) <= ε * (val_size + 1))%R ->
-    hash_tape α ns γ3 -∗
-    ↯ ε -∗
-    hash_set s γ3 -∗
-    state_update E E (∃ (n:fin (S val_size)),
-          hash_tape α (ns++[fin_to_nat n]) γ3 ∗
-          ( (⌜fin_to_nat n ∈ s⌝) ∗ hash_set s γ3 ∗ ↯ εI ∨
-            (⌜fin_to_nat n ∉ s⌝) ∗ hash_set (s∪{[(fin_to_nat n)]}) γ3 ∗ ↯ εO
-          )
+    hash_tape_auth m γ_set γ -∗ hash_tape α ns γ_set γ -∗ ↯ ε -∗
+    hash_set s γ_set -∗
+    state_update E E (∃ (n:fin(S val_size)), 
+          ( (⌜fin_to_nat n ∈ s⌝) ∗ hash_set s γ_set ∗ ↯ εI  ∨
+            (⌜fin_to_nat n ∉ s⌝) ∗ hash_set (s∪{[(fin_to_nat n)]}) γ_set ∗ ↯ εO
+          )∗
+          hash_tape_auth (<[α:=ns++[fin_to_nat n]]>m) γ_set γ ∗
+          hash_tape α (ns++[fin_to_nat n]) γ_set γ
       ).
   Proof.
-    iIntros (Hineq) "Ht Herr Hs".
+    iIntros (Hineq) "[Htauth #?] [Ht #?] Herr (Hs&%&#?)".
     pose (ε2 (x:fin (S val_size)):= if bool_decide (fin_to_nat x ∈s) then nonneg εI else nonneg εO).
-    rewrite /hash_tape/hash_set.
-    iDestruct "Ht" as "[Ht #Hfrag]".
-    iDestruct "Hs" as "[Hs [% #Hfrags]]".
-    iMod (rand_tapes_presample _ _ _ _ _ ε2 with "[$][$]") as (n) "[Herr Htape]". 
+    iMod (con_hash_interface0.hash_tape_presample _ _ _ _ _ ε2 with "[$][$][$]") as "(%&Herr&Htauth&Ht)".
     - intros. rewrite /ε2. case_bool_decide; apply cond_nonneg.
     - rewrite /ε2.
       (** copied from error rules *)
@@ -222,215 +205,382 @@ Section con_hash_impl1.
       apply Rcomplements.Rle_div_l; [lra |].
       rewrite SeriesC_fin_in_set; auto.
       rewrite SeriesC_fin_not_in_set; auto.
-    - rewrite /ε2.
-      case_bool_decide as Hin.
-      + iModIntro. iFrame "Htape".
-        iSplitR.
-        * iSplit; first done.
+    - iFrame. rewrite /ε2. case_bool_decide.
+      + iModIntro. repeat iSplit; try done.
+        * iLeft. iFrame. by repeat iSplit.
+        * iApply big_sepM_insert_2; last done.
+          iSplit; first done.
           iSplit; last done.
-          by iDestruct (big_sepS_elem_of with "[$Hfrags]") as "$".
-        * iLeft. iFrame. iFrame "Hfrags".
-          iPureIntro. naive_solver.
-      + iMod (ghost_map_insert_persist (fin_to_nat n) with "[$]") as "[Hs #?]".
+          by iApply (big_sepS_elem_of with "[$]").
+        * by iApply (big_sepS_elem_of with "[$]").
+      + iMod (ghost_map_insert_persist (fin_to_nat n) with "[$]") as "[Hs #?]". 
         * by rewrite lookup_gset_to_gmap_None.
-        * iModIntro. iFrame "Htape".
-          iSplitR.
-          -- iSplit; first done. by iSplit.
-          -- iRight. iFrame. repeat iSplit.
-             ++ done.
-             ++ rewrite -gset_to_gmap_union_singleton.
+        * iModIntro. repeat iSplit; try done.
+          -- iRight. iFrame.
+             iSplit; first done. repeat iSplit.
+             ++ rewrite <-gset_to_gmap_union_singleton.
                 by rewrite union_comm_L.
              ++ iPureIntro.
                 set_unfold. intros ? [|]; first naive_solver.
                 subst.
                 apply fin_to_nat_lt.
              ++ by iApply big_sepS_insert_2'.
+          -- iApply big_sepM_insert_2; last done.
+             iSplit; first done.
+             by iSplit.
   Qed.
 
-  Lemma con_hash_init:
-    {{{ True }}}
-      init_hash #()
-      {{{ (f:val), RET f; ∃ l hm γ1 γ3 γ_lock, con_hash_inv f l hm γ1 γ3 γ_lock ∗
-                                                  hash_set ∅ γ3
-      }}}.
-  Proof.
-    iIntros (Φ) "_ HΦ".
-    iMod (ghost_map_alloc_empty) as (γ3) "H3".
-    rewrite /init_hash.
-    wp_pures.
-    rewrite /con_hash_inv/abstract_con_hash_inv/abstract_con_hash/concrete_con_hash_inv/concrete_con_hash.
-    rewrite /init_hash_state.
-    wp_apply (wp_init_map with "[$]") as (l) "Hm".
-    wp_pures.
-    iMod (ghost_var_alloc ∅) as "[%γ2 [Hauth Hfrag]]".
-    wp_apply (newlock_spec with "[Hm Hfrag]") as (loc γ_lock) "#Hl"; last first.
-    - wp_pures. 
-      iMod hv_auth_init as "[%γ1 Hv]".
-      iMod (inv_alloc with "[Hauth Hv]") as "#Hinv"; last first.
-      + rewrite /compute_con_hash. wp_pures.  iApply "HΦ". iFrame "Hinv Hl".
-        rewrite /hash_set. rewrite gset_to_gmap_empty. iFrame. iModIntro.
-        by iSplit. 
-      + rewrite /compute_con_hash_specialized. iFrame. iNext. by iSplit. 
-    - by iFrame.
+  Lemma con_hash_presample  N f l hm P {HP: ∀ m m', Timeless (P m m')} γ_hv γ_set γ_tape γ_lock Q
+    E  :
+    ↑N ⊆ E ->
+    con_hash_inv N f l hm P γ_hv γ_set γ_tape γ_lock -∗
+    (∀ m m', P m m'  -∗
+             hash_tape_auth m' γ_set γ_tape -∗
+             state_update (E∖↑N) (E∖↑N)
+             (∃ m'', P m m'' ∗ hash_tape_auth m'' γ_set γ_tape ∗ Q m m' m'')
+    ) -∗
+    state_update E E (
+        ∃ m m' m'', Q m m' m''
+      ) .
+  Proof. 
+    iIntros (Hsubset) "#Hinv Hvs".
+    iMod (con_hash_presample0 with "[//][-]"); first done; last done.
+    iIntros (m m') "[[Hauth #?][#?HP]] Ht".
+    rewrite /hash_tape_auth.
+    iMod ("Hvs" with "[$][$Ht]") as "(%&HP&[Ht #?]&HQ)"; first done.
+    iFrame. iModIntro. by iSplit.
   Qed.
+
+  (* Lemma con_hash_presample N f l hm P {HP: ∀ m m', Timeless (P m m')} γ1 γ2 γ_lock Q *)
+  (*   E (ε εI εO:nonnegreal) ns α  s: *)
+  (*   ↑N ⊆ E -> *)
+  (*   (εI * (size s) + εO * (val_size + 1 - size s) <= ε * (val_size + 1))%R -> *)
+  (*   con_hash_inv N f l hm P γ1 γ2 γ_lock -∗ *)
+  (*   (∀ m m' n, P m m'  -∗ *)
+  (*            ⌜m'!!α=Some ns⌝ ∗ *)
+  (*            |={E∖↑N}=> *)
+  (*              (P m (<[α:=ns++[fin_to_nat n]]> m') ∗ *)
+  (*                  Q n *)
+  (*              ) *)
+  (*   ) -∗ *)
+  (*   hash_set s γ2 -∗ *)
+  (*   hash_tape α ns γ2 -∗ *)
+  (*   ↯ ε -∗ *)
+  (*   state_update E E (∃ (n:fin (S val_size)), *)
+  (*         ( (⌜fin_to_nat n ∈ s⌝) ∗ hash_set s γ2 ∗ ↯ εI ∨ *)
+  (*           (⌜fin_to_nat n ∉ s⌝) ∗ hash_set (s∪{[(fin_to_nat n)]}) γ2 ∗ ↯ εO *)
+  (*         ) ∗ *)
+  (*         hash_tape α (ns++[fin_to_nat n]) γ2∗ *)
+  (*         Q n *)
+  (*     ). *)
+  (* Proof. *)
+  (*   iIntros (Hsubset Hineq) "#Hinv Hvs Hs Htape Herr". *)
+  (*   pose (ε2 (x:fin (S val_size)):= if bool_decide (fin_to_nat x ∈s) then nonneg εI else nonneg εO). *)
+  (*   iDestruct "Htape" as "[Htape #?]". *)
+  (*   iDestruct "Hs" as "(?&%&#?)". *)
+  (*   iMod (con_hash_presample0 _ _ _ _ _ _ Q _ _ _ _ ε2 with "[//][Hvs][$][$]") as "(%n&Herr&Htape&HQ)". *)
+  (*   - done. *)
+  (*   - intros. rewrite /ε2. case_bool_decide; apply cond_nonneg. *)
+  (*   - rewrite /ε2. *)
+  (*     (** copied from error rules *) *)
+  (*     rewrite S_INR. *)
+  (*     rewrite SeriesC_scal_l. *)
+  (*     rewrite (SeriesC_ext _ (λ x : fin (S val_size), *)
+  (*                               εI * (if bool_decide (fin_to_nat x ∈ s) then 1 else 0) + *)
+  (*                                 εO * (if bool_decide (¬(fin_to_nat x ∈ s)) then 1 else 0))%R); last first. *)
+  (*     { *)
+  (*       intro n. *)
+  (*       case_bool_decide as HE ; case_bool_decide as HF; simpl. *)
+  (*       - done. *)
+  (*       - lra. *)
+  (*       - lra. *)
+  (*       - done. *)
+  (*     } *)
+  (*     rewrite SeriesC_plus; [ | apply ex_seriesC_finite | apply ex_seriesC_finite]. *)
+  (*     rewrite 2!SeriesC_scal_l. *)
+  (*     rewrite /Rdiv Rmult_1_l. *)
+  (*     rewrite Rmult_comm. *)
+  (*     rewrite -Rdiv_def. *)
+  (*     pose proof (pos_INR val_size). *)
+  (*     apply Rcomplements.Rle_div_l; [lra |]. *)
+  (*     rewrite SeriesC_fin_in_set; auto. *)
+  (*     rewrite SeriesC_fin_not_in_set; auto. *)
+  (*   - iIntros (m m' n) "[Hauth HP]". *)
+  (*     iDestruct ("Hvs" with "[$]") as "[% Hvs]". *)
+  (*     iSplit; first done. *)
+  (*     iMod "Hvs". by iFrame. *)
+  (*   - rewrite /ε2. case_bool_decide as Heqn.  *)
+  (*     + iFrame. iModIntro. iSplit. *)
+  (*       * iLeft. iFrame. by repeat iSplit. *)
+  (*       * iSplit; first done. iSplit; last done. *)
+  (*         by iApply (big_sepS_elem_of with "[//]"). *)
+  (*     + iMod (ghost_map_insert_persist (fin_to_nat n) with "[$]") as "[Hs #?]". *)
+  (*       * by rewrite lookup_gset_to_gmap_None. *)
+  (*       * iModIntro. iFrame "Htape". *)
+  (*         iFrame. iSplit. *)
+  (*         -- iRight. iFrame. *)
+  (*            iSplit; first done. repeat iSplit. *)
+  (*            ++ rewrite <-gset_to_gmap_union_singleton. *)
+  (*               by rewrite union_comm_L. *)
+  (*            ++ iPureIntro. *)
+  (*               set_unfold. intros ? [|]; first naive_solver. *)
+  (*               subst. *)
+  (*               apply fin_to_nat_lt. *)
+  (*            ++ by iApply big_sepS_insert_2'. *)
+  (*         -- by repeat iSplit. *)
+  (* Qed. *)
+          
+
+  (* Lemma con_hash_init N P {HP: ∀ m m', Timeless (P m m')}: *)
+  (*   {{{ P ∅ ∅ }}} *)
+  (*     init_hash #() *)
+  (*     {{{ (f:val), RET f; ∃ l hm γ1 γ2 γ_lock, con_hash_inv N f l hm P γ1 γ2 γ_lock ∗ *)
+  (*                                                 hash_set ∅ γ2 *)
+  (*     }}}. *)
+  (* Proof. *)
+  (*   iIntros (Φ) "HP HΦ". *)
+  (*   iMod hv_auth_init as "[%γ1 Hv]".   *)
+  (*   iMod (ghost_map_alloc_empty) as (γ2) "H2". *)
+  (*   rewrite /init_hash. *)
+  (*   rewrite /con_hash_inv. *)
+  (*   wp_apply (con_hash_init0 _ (λ (m : gmap nat nat) (m' : gmap val (list nat)), hash_auth m γ1 γ2 ∗ P m m')%I with "[$HP $Hv]"); first done. *)
+  (*   iIntros (f) "(%&%&%&#Hinv)". *)
+  (*   iApply "HΦ". *)
+  (*   iFrame "Hinv". iFrame. by repeat iSplit. *)
+  (* Qed. *)
   
 
-  Lemma con_hash_alloc_tape f l hm γ1 γ3 γ_lock:
-    {{{ con_hash_inv f l hm γ1 γ3 γ_lock }}}
-      allocate_tape #()
-      {{{ (α: val), RET α; hash_tape α [] γ3 }}}.
-  Proof.
-    rewrite /hash_tape.
-    iIntros (Φ) "_ HΦ".
-    rewrite /allocate_tape.
-    wp_pures.
-    wp_apply (rand_allocate_tape_spec with "[//]") as (v) "?".
-    iApply "HΦ".
-    by iFrame.
-  Qed.
+  (* Lemma con_hash_alloc_tape N f l hm P {HP: ∀ m m', Timeless (P m m')} γ1 γ2 γ_lock Q: *)
+  (* {{{ con_hash_inv N f l hm P γ1 γ2 γ_lock ∗ *)
+  (*     (∀ m m' α, P m m' -∗ ⌜α∉dom m'⌝ ∗ |={⊤∖↑N}=> P m (<[α:=[]]>m') ∗ Q α) *)
+  (* }}} *)
+  (*     allocate_tape #() *)
+  (*     {{{ (α: val), RET α; hash_tape α [] γ2 ∗ Q α }}}. *)
+  (* Proof. *)
+  (*   rewrite /hash_tape. *)
+  (*   iIntros (Φ) "[#Hinv Hvs] HΦ". *)
+  (*   rewrite /allocate_tape. *)
+  (*   rewrite /con_hash_inv. *)
+  (*   wp_apply (con_hash_alloc_tape0 _ _ _ _ _ _ Q with "[$Hinv Hvs][HΦ]"). *)
+  (*   - iIntros (???) "[Hauth HP]". *)
+  (*     iDestruct ("Hvs" with "[$]") as "[% Hvs]". *)
+  (*     iSplit; first done. *)
+  (*     iMod "Hvs". by iFrame. *)
+  (*   - iNext. iIntros (?) "[??]". *)
+  (*     iApply "HΦ". *)
+  (*     by iFrame. *)
+  (* Qed. *)
 
-  Lemma con_hash_spec f l hm γ1 γ3 γlock α n ns (v:nat):
-    {{{ con_hash_inv f l hm γ1 γ3 γlock ∗ hash_tape α (n::ns) γ3 }}}
-      f #v α
-      {{{ (res:nat), RET (#res);  con_hash_view v res γ1 γ3 ∗
-                                (hash_tape α ns γ3 ∗ ⌜res=n⌝ ∨
-                                 hash_tape α (n::ns) γ3
-                                )
-      }}}.
-  Proof.
-    rewrite /con_hash_inv/hash_tape.
-    iIntros (Φ) "[[%γ2 #[Hab Hcon]] [Ht #Hfrag1]] HΦ".
-    iApply pgl_wp_fupd.
-    iApply fupd_pgl_wp.
-    iInv "Hab" as ">(%&->&H1&H2)" "Hclose".
-    iMod ("Hclose" with "[$H1 $H2]") as "_"; first done.
-    iModIntro.
-    rewrite /compute_con_hash_specialized.
-    wp_pures.
-    wp_apply (acquire_spec with "Hcon") as "[Hl[% (%&->&Hm&Hfrag)]]".
-    wp_pures.
-    rewrite /compute_hash.
-    wp_pures.
-    wp_apply (wp_get with "[$]") as (res) "[Hm ->]".
-    rewrite lookup_fmap.
-    destruct (_!!_) eqn:Hres; simpl.
-    - (* hashed before *)
-      wp_pures.
-      iApply fupd_pgl_wp.
-      iInv "Hab" as ">(%&->&H1&H2&#Hfrag2)" "Hclose".
-      iDestruct (ghost_var_agree with "[$][$]") as "->".
-      iDestruct (hv_auth_duplicate_frag with "[$]") as "[H1 Hfrag']"; first done.
-      iMod ("Hclose" with "[$H1 $H2]") as "_"; first by iSplit.
-      iModIntro.
-      wp_apply (release_spec with "[$Hl $Hcon $Hfrag $Hm]") as "_"; first done.
-      wp_pures.
-      iModIntro. iApply "HΦ".
-      iFrame.
-      iSplit.
-      + by iDestruct (big_sepM_lookup with "[$]") as "?".
-      + iRight. by iFrame. 
-    - wp_pures.
-      rewrite /hash_tape.
-      wp_apply (rand_tape_spec_some with "[$]") as "Ht".
-      wp_pures.
-      wp_apply (wp_set with "[$]") as "Hm".
-      iApply fupd_pgl_wp.
-      iInv "Hab" as ">(%&->&H1&H2& #Hfrag2)" "Hclose".
-      iDestruct (ghost_var_agree with "[$][$]") as "->".
-      iMod (ghost_var_update _ (<[v:=n]> _) with "[$][$]") as "[H2 Hfrag]".
-      iMod (hv_auth_insert with "[$]") as "[H1 Hfrag']"; first done.
-      iMod ("Hclose" with "[$H1 $H2]") as "_".
-      { iSplit; first done.
-        iNext. rewrite big_sepM_insert; last done.
-        iFrame "Hfrag2".
-        by iDestruct "Hfrag1" as "[??]".
-      }
-      iModIntro.
-      wp_pures.
-      wp_apply (release_spec with "[$Hl $Hcon $Hfrag Hm]") as "_".
-      { iExists _. iSplit; first done. by rewrite fmap_insert. }
-      wp_pures.
-      iApply "HΦ".
-      iFrame. iModIntro.
-      iDestruct "Hfrag1" as "[??]".
-      iSplit; first done.
-      iLeft. iFrame. by iSplit.
-  Qed.
+  (* Lemma con_hash_spec N f l hm P {HP: ∀ m m', Timeless (P m m')} γ1 γ2 γ_lock Q1 Q2 α ns (v:nat): *)
+  (* {{{ con_hash_inv N f l hm P γ1 γ2 γ_lock ∗ hash_tape α (ns) γ2 ∗ *)
+  (*     ( ∀ m m', hash_auth m γ1 γ2 -∗ P m m' -∗ ⌜m'!!α=Some ns⌝ ∗ |={⊤∖↑N}=> *)
+  (*            match m!!v with *)
+  (*            | Some res => hash_auth m γ1 γ2 ∗ P m m' ∗ Q1 res *)
+  (*            | None => ∃ n ns', ⌜n::ns'=ns⌝ ∗ hash_auth (<[v:=n]> m) γ1 γ2 ∗ P (<[v:=n]> m) (<[α:=ns']> m') ∗ Q2 *)
+  (*            end                                         *)
+  (*     ) *)
+  (* }}} *)
+  (*     f #v α *)
+  (*     {{{ (res:nat), RET (#res);  (hash_tape α (ns) γ2 ∗ Q1 res ∨ *)
+  (*                                ∃ n ns', ⌜n::ns'=ns⌝ ∗ hash_tape α ns' γ2 ∗ ⌜res=n⌝ ∗ Q2  *)
+  (*                               ) *)
+  (*     }}}. *)
+  (* Proof. *)
+  (*   rewrite /con_hash_inv. *)
+  (*   iIntros (Φ) "(#Hinv & Htape & Hvs) HΦ". *)
+  (*   iDestruct "Htape" as "[Htape #Hfrag]". *)
+  (*   wp_apply (con_hash_spec0 _ _ _ _ _ _ Q1 Q2 with "[$Hinv Hvs $Htape]"). *)
+  (*   - iIntros (m m') "[Hauth HP]". *)
+  (*     iDestruct ("Hvs" with "[$][$]") as "[% Hvs]". *)
+  (*     iSplit; first done. *)
+  (*     iMod "Hvs". case_match. *)
+  (*     + by iDestruct "Hvs" as "($ &$&$)". *)
+  (*     + by iDestruct "Hvs" as "(%&%&<-&$&$&$)". *)
+  (*   - iIntros (res) "[[Ht HQ]|(%&%&<-&?&->&H)]"; iApply "HΦ". *)
+  (*     + iLeft. by iFrame. *)
+  (*     + iRight. iFrame. iExists _. repeat iSplit; try done. *)
+  (*       rewrite big_sepL_cons. iDestruct "Hfrag" as "[_ $]". *)
+  (* Qed.  *)
 
-  Lemma con_hash_spec_hashed_before f l hm γ1 γ3 γlock α ns res (v:nat):
-    {{{ con_hash_inv f l hm γ1 γ3 γlock ∗ hash_tape α ns γ3 ∗ con_hash_view v res γ1 γ3 }}}
-      f #v α
-      {{{ RET (#res);  con_hash_view v res γ1 γ3 ∗
-                       (hash_tape α ns γ3 )
-      }}}.
-  Proof.
-    iIntros (Φ) "[[%γ2 [#Hab #Hcon]][Ht #[Hfragv Hfragv']]] HΦ".
-    rewrite /abstract_con_hash_inv/concrete_con_hash_inv.
-    iApply fupd_pgl_wp.
-    iInv "Hab" as ">(%&->&H1&H2)" "Hclose".
-    iMod ("Hclose" with "[$H1 $H2]") as "_"; first done.
-    iModIntro.
-    rewrite /compute_con_hash_specialized.
-    wp_pures.
-    wp_apply (acquire_spec with "Hcon") as "[Hl[% (%&->&Hm&Hfrag)]]".
-    wp_pures.
-    rewrite /compute_hash.
-    wp_pures.
-    wp_apply (wp_get with "[$]") as (res') "[Hm ->]".
-    rewrite lookup_fmap.
-    destruct (_!!_) eqn:Hres; simpl.
-    - (* hashed before *)
-      wp_pures.
-      iApply fupd_pgl_wp.
-      iInv "Hab" as ">(%&->&H1&H2&#Hfrag')" "Hclose".
-      iDestruct (ghost_var_agree with "[$][$]") as "->".
-      iDestruct (hv_auth_frag_agree with "[$]") as "%H".
-      rewrite Hres in H. simplify_eq.
-      iMod ("Hclose" with "[$H1 $H2]") as "_"; first by iSplit.
-      iModIntro.
-      wp_apply (release_spec with "[$Hl $Hcon $Hfrag $Hm]") as "_"; first done.
-      wp_pures. iModIntro.
-      iApply "HΦ".
-      iFrame. rewrite /con_hash_view. iFrame "Hfragv Hfragv'". 
-    - iApply fupd_pgl_wp.
-      iInv "Hab" as ">(%&->&H1&H2&#?)" "Hclose".
-      iDestruct (ghost_var_agree with "[$][$]") as "->".
-      iDestruct (hv_auth_frag_agree with "[$]") as "%H". simplify_eq.
-  Qed.
 
-  Program Definition con_hash_impl1 : con_hash1 val_size :=
-    {| init_hash1:=init_hash;
-      allocate_tape1:=allocate_tape;
-      compute_hash1:=compute_hash;
+  (* Program Definition con_hash_impl1 : con_hash1 val_size := *)
+  (*   {| init_hash1:=init_hash; *)
+  (*     allocate_tape1:=allocate_tape; *)
+  (*     compute_hash1:=compute_hash; *)
 
-      hash_view_gname:=_;
-      hash_lock_gname:=_;
-      con_hash_inv1 := con_hash_inv;
-      hash_tape1:=hash_tape;
-      con_hash_view1:=con_hash_view;
-      con_hash_presample1 := con_hash_presample;
-      con_hash_init1 := con_hash_init;
-      con_hash_alloc_tape1 := con_hash_alloc_tape;
-      con_hash_spec1 := con_hash_spec;
-      con_hash_spec_hashed_before1 := con_hash_spec_hashed_before                
-    |}
-  .
-  Next Obligation.
-    rewrite /con_hash_view.
-    iIntros (?????) "[??][??]".
-    by iDestruct (hv_frag_frag_agree with "[$][$]") as "->".
-  Qed.
-  Next Obligation.
-    iIntros.
-    by iApply con_hash_view_in_hash_set.
-  Qed.
-  Next Obligation.
-    iIntros (????) "[??]?".
-    by iApply (tape_in_hash_set with "[$]").
-  Qed.
-  Next Obligation.
-    iIntros (???) "[??]".
-    by iApply rand_tapes_valid.
-  Qed.
+  (*     hash_view_gname:=_; *)
+  (*     hash_set_gname:=_; *)
+  (*     hash_lock_gname:=_; *)
+      
+  (*     con_hash_inv1 := con_hash_inv; *)
+  (*     hash_tape1:=hash_tape; *)
+  (*     hash_frag1:=hash_frag; *)
+  (*     hash_auth1:=hash_auth; *)
+  (*     hash_set1:=hash_set; *)
+  (*     hash_set_frag1:=hash_set_frag; *)
+  (*     con_hash_presample1 := con_hash_presample; *)
+  (*     con_hash_init1 := con_hash_init; *)
+  (*     con_hash_alloc_tape1 := con_hash_alloc_tape; *)
+  (*     con_hash_spec1:=con_hash_spec *)
+  (*   |} *)
+  (* . *)
+  (* Next Obligation. *)
+  (*   iIntros (????) "[??][??]". *)
+  (*   iApply (hv_auth_exclusive with "[$][$]"). *)
+  (* Qed. *)
+  (* Next Obligation. *)
+  (*   iIntros (?????)"[??][??]". *)
+  (*   iApply (hv_auth_frag_agree with "[$]"). *)
+  (* Qed. *)
+  (* Next Obligation. *)
+  (*   iIntros (??????) "[??]". *)
+  (*   iDestruct (hv_auth_duplicate_frag with "[$]") as "[? $]"; first done. *)
+  (*   by iApply (big_sepM_lookup with "[$]"). *)
+  (* Qed. *)
+  (* Next Obligation. *)
+  (*   rewrite /hash_frag. *)
+  (*   iIntros (?????) "[??][??]". *)
+  (*   by iDestruct (hv_frag_frag_agree with "[$][$]") as "->". *)
+  (* Qed. *)
+  (* Next Obligation. *)
+  (*   iIntros (????) "[?$]". *)
+  (* Qed. *)
+  (* Next Obligation. *)
+  (*   iIntros (???) "[?#$]". *)
+  (* Qed. *)
+  (* Next Obligation. *)
+  (*   iIntros (???) "[H1 ?]H2". *)
+  (*   iCombine "H1 H2" gives "%H". *)
+  (*   iPureIntro. *)
+  (*   rewrite lookup_gset_to_gmap_Some in H. naive_solver. *)
+  (* Qed. *)
+  (* Next Obligation. *)
+  (*   iIntros (??????) "?[??]". *)
+  (*   rewrite /hash_auth. *)
+  (*   iMod (hv_auth_insert with "[$]") as "[$ ?]"; first done. *)
+  (*   iModIntro. *)
+  (*   rewrite big_sepM_insert; last done. iFrame. *)
+  (* Qed. *)
+  (* Next Obligation. *)
+  (*   iIntros (??)"(?&%H&?)". iPureIntro. intros n H'. *)
+  (*   apply H in H'. lia. *)
+  (* Qed. *)
+  (* Next Obligation. *)
+  (*   iIntros (???) "[??]". *)
+  (*   by iApply con_hash_interface0.hash_tape_valid. *)
+  (* Qed. *)
+  (* Next Obligation. *)
+  (*   iIntros (????) "[H1 _] [H2 _]". *)
+  (*   iApply (con_hash_interface0.hash_tape_exclusive with "[$][$]"). *)
+  (* Qed. *)
   
 End con_hash_impl1.
+
+  (* Lemma con_hash_spec f l hm γ1 γ3 γlock α n ns (v:nat): *)
+  (*   {{{ con_hash_inv f l hm γ1 γ3 γlock ∗ hash_tape α (n::ns) γ3 }}} *)
+  (*     f #v α *)
+  (*     {{{ (res:nat), RET (#res);  hash_frag v res γ1 γ3 ∗ *)
+  (*                               (hash_tape α ns γ3 ∗ ⌜res=n⌝ ∨ *)
+  (*                                hash_tape α (n::ns) γ3 *)
+  (*                               ) *)
+  (*     }}}. *)
+  (* Proof. *)
+  (*   rewrite /con_hash_inv/hash_tape. *)
+  (*   iIntros (Φ) "[[%γ2 #[Hab Hcon]] [Ht #Hfrag1]] HΦ". *)
+  (*   iApply pgl_wp_fupd. *)
+  (*   iApply fupd_pgl_wp. *)
+  (*   iInv "Hab" as ">(%&->&H1&H2)" "Hclose". *)
+  (*   iMod ("Hclose" with "[$H1 $H2]") as "_"; first done. *)
+  (*   iModIntro. *)
+  (*   rewrite /compute_con_hash_specialized. *)
+  (*   wp_pures. *)
+  (*   wp_apply (acquire_spec with "Hcon") as "[Hl[% (%&->&Hm&Hfrag)]]". *)
+  (*   wp_pures. *)
+  (*   rewrite /compute_hash. *)
+  (*   wp_pures. *)
+  (*   wp_apply (wp_get with "[$]") as (res) "[Hm ->]". *)
+  (*   rewrite lookup_fmap. *)
+  (*   destruct (_!!_) eqn:Hres; simpl. *)
+  (*   - (* hashed before *) *)
+  (*     wp_pures. *)
+  (*     iApply fupd_pgl_wp. *)
+  (*     iInv "Hab" as ">(%&->&H1&H2&#Hfrag2)" "Hclose". *)
+  (*     iDestruct (ghost_var_agree with "[$][$]") as "->". *)
+  (*     iDestruct (hv_auth_duplicate_frag with "[$]") as "[H1 Hfrag']"; first done. *)
+  (*     iMod ("Hclose" with "[$H1 $H2]") as "_"; first by iSplit. *)
+  (*     iModIntro. *)
+  (*     wp_apply (release_spec with "[$Hl $Hcon $Hfrag $Hm]") as "_"; first done. *)
+  (*     wp_pures. *)
+  (*     iModIntro. iApply "HΦ". *)
+  (*     iFrame. *)
+  (*     iSplit. *)
+  (*     + by iDestruct (big_sepM_lookup with "[$]") as "?". *)
+  (*     + iRight. by iFrame.  *)
+  (*   - wp_pures. *)
+  (*     rewrite /hash_tape. *)
+  (*     wp_apply (rand_tape_spec_some with "[$]") as "Ht". *)
+  (*     wp_pures. *)
+  (*     wp_apply (wp_set with "[$]") as "Hm". *)
+  (*     iApply fupd_pgl_wp. *)
+  (*     iInv "Hab" as ">(%&->&H1&H2& #Hfrag2)" "Hclose". *)
+  (*     iDestruct (ghost_var_agree with "[$][$]") as "->". *)
+  (*     iMod (ghost_var_update _ (<[v:=n]> _) with "[$][$]") as "[H2 Hfrag]". *)
+  (*     iMod (hv_auth_insert with "[$]") as "[H1 Hfrag']"; first done. *)
+  (*     iMod ("Hclose" with "[$H1 $H2]") as "_". *)
+  (*     { iSplit; first done. *)
+  (*       iNext. rewrite big_sepM_insert; last done. *)
+  (*       iFrame "Hfrag2". *)
+  (*       by iDestruct "Hfrag1" as "[??]". *)
+  (*     } *)
+  (*     iModIntro. *)
+  (*     wp_pures. *)
+  (*     wp_apply (release_spec with "[$Hl $Hcon $Hfrag Hm]") as "_". *)
+  (*     { iExists _. iSplit; first done. by rewrite fmap_insert. } *)
+  (*     wp_pures. *)
+  (*     iApply "HΦ". *)
+  (*     iFrame. iModIntro. *)
+  (*     iDestruct "Hfrag1" as "[??]". *)
+  (*     iSplit; first done. *)
+  (*     iLeft. iFrame. by iSplit. *)
+  (* Qed. *)
+
+  (* Lemma con_hash_spec_hashed_before f l hm γ1 γ3 γlock α ns res (v:nat): *)
+  (*   {{{ con_hash_inv f l hm γ1 γ3 γlock ∗ hash_tape α ns γ3 ∗ hash_frag v res γ1 γ3 }}} *)
+  (*     f #v α *)
+  (*     {{{ RET (#res);  hash_frag v res γ1 γ3 ∗ *)
+  (*                      (hash_tape α ns γ3 ) *)
+  (*     }}}. *)
+  (* Proof. *)
+  (*   iIntros (Φ) "[[%γ2 [#Hab #Hcon]][Ht #[Hfragv Hfragv']]] HΦ". *)
+  (*   rewrite /abstract_con_hash_inv/concrete_con_hash_inv. *)
+  (*   iApply fupd_pgl_wp. *)
+  (*   iInv "Hab" as ">(%&->&H1&H2)" "Hclose". *)
+  (*   iMod ("Hclose" with "[$H1 $H2]") as "_"; first done. *)
+  (*   iModIntro. *)
+  (*   rewrite /compute_con_hash_specialized. *)
+  (*   wp_pures. *)
+  (*   wp_apply (acquire_spec with "Hcon") as "[Hl[% (%&->&Hm&Hfrag)]]". *)
+  (*   wp_pures. *)
+  (*   rewrite /compute_hash. *)
+  (*   wp_pures. *)
+  (*   wp_apply (wp_get with "[$]") as (res') "[Hm ->]". *)
+  (*   rewrite lookup_fmap. *)
+  (*   destruct (_!!_) eqn:Hres; simpl. *)
+  (*   - (* hashed before *) *)
+  (*     wp_pures. *)
+  (*     iApply fupd_pgl_wp. *)
+  (*     iInv "Hab" as ">(%&->&H1&H2&#Hfrag')" "Hclose". *)
+  (*     iDestruct (ghost_var_agree with "[$][$]") as "->". *)
+  (*     iDestruct (hv_auth_frag_agree with "[$]") as "%H". *)
+  (*     rewrite Hres in H. simplify_eq. *)
+  (*     iMod ("Hclose" with "[$H1 $H2]") as "_"; first by iSplit. *)
+  (*     iModIntro. *)
+  (*     wp_apply (release_spec with "[$Hl $Hcon $Hfrag $Hm]") as "_"; first done. *)
+  (*     wp_pures. iModIntro. *)
+  (*     iApply "HΦ". *)
+  (*     iFrame. rewrite /hash_frag. iFrame "Hfragv Hfragv'".  *)
+  (*   - iApply fupd_pgl_wp. *)
+  (*     iInv "Hab" as ">(%&->&H1&H2&#?)" "Hclose". *)
+  (*     iDestruct (ghost_var_agree with "[$][$]") as "->". *)
+  (*     iDestruct (hv_auth_frag_agree with "[$]") as "%H". simplify_eq. *)
+  (* Qed. *)
