theories/coneris/examples/hash/con_hash_interface0.v
@@ -2,9 +2,6 @@ From clutch.coneris Require Import coneris .
 
 Set Default Proof Using "Type*".
 
-(** This spec is not strong enough to say anything about how the value hashed must be somthing we presampled
-    For that info, please refer to interface1
-*)
 
 Class con_hash0 `{!conerisGS Σ} (val_size:nat):= Con_Hash0
 {
@@ -18,76 +15,99 @@ Class con_hash0 `{!conerisGS Σ} (val_size:nat):= Con_Hash0
   (** [name] is used to associate [locked] with [is_lock] *)
   (* tape_name: Type; *)
   
-  hash_view_gname:Type;
+  (* hash_view_gname:Type; *)
+  hash_tape_gname: Type;
   hash_lock_gname:Type;
   
   (** * Predicates *)
-  con_hash_inv0 (N:namespace) (f l hm: val) (γ1:hash_view_gname)(γ_lock:hash_lock_gname): iProp Σ;
+  con_hash_inv0 (N:namespace) (f l hm: val) (P:gmap nat nat -> gmap val (list nat) -> iProp Σ) {HP: ∀ m m', Timeless (P m m')} (γ:hash_tape_gname) (γ_lock:hash_lock_gname): iProp Σ;
   (* concrete_seq_hash {L:seq_hashG Σ} (f:val) (m:gmap nat nat) : iProp Σ;  *)
-  hash_tape0 (α:val) (ns:list nat) : iProp Σ;
-  hash_auth0 (m:gmap nat nat) (γ2:hash_view_gname) : iProp Σ;
-  hash_frag0 (v res:nat) (γ:hash_view_gname): iProp Σ;
+  hash_tape0 (α:val) (ns:list nat) (γ:hash_tape_gname): iProp Σ;
+  hash_tape_auth0 (m:gmap val (list nat)) (γ:hash_tape_gname) :iProp Σ;
+  (* hash_auth0 (m:gmap nat nat) (γ2:hash_view_gname) : iProp Σ; *)
+  (* hash_frag0 (v res:nat) (γ:hash_view_gname): iProp Σ; *)
   
   (** * General properties of the predicates *)
-  (* #[global] concrete_seq_hash_timeless {L : seq_hashG Σ} f m :: *)
-  (*   Timeless (concrete_seq_hash (L:=L) f m); *)
-  #[global] hash_tape_timeless α ns ::
-    Timeless (hash_tape0 α ns); 
-  #[global] hash_map_timeless m γ ::
-    Timeless (hash_auth0 m γ);
-  #[global] hash_frag_timeless v res γ ::
-    Timeless (hash_frag0 v res γ);
-  #[global] con_hash_inv_persistent N f l hm γ1 γ_lock ::
-    Persistent (con_hash_inv0 N f l hm γ1 γ_lock);
-  #[global] hash_frag_persistent v res γ ::
-    Persistent (hash_frag0 v res γ);
+  #[global] hash_tape_timeless α ns γ::
+    Timeless (hash_tape0 α ns γ); 
+  #[global] hash_tape_auth_timeless m γ::
+    Timeless (hash_tape_auth0 m γ);
+  (* #[global] hash_map_timeless m γ :: *)
+  (*   Timeless (hash_auth0 m γ); *)
+  (* #[global] hash_frag_timeless v res γ :: *)
+  (*   Timeless (hash_frag0 v res γ); *)
+  #[global] con_hash_inv_persistent N f l hm P {HP: ∀ m m', Timeless (P m m')} γ_tape γ_lock ::
+    Persistent (con_hash_inv0 N f l hm P γ_tape γ_lock); 
+  (* #[global] hash_frag_persistent v res γ :: *)
+  (*   Persistent (hash_frag0 v res γ); *)
   
-  hash_tape_valid α ns:
-    hash_tape0 α ns -∗ ⌜Forall (λ x, x<=val_size)%nat ns⌝;
-  hash_auth_exclusive m m' γ:
-    hash_auth0 m γ -∗ hash_auth0 m' γ -∗ False;
-  hash_auth_frag_agree m k v γ:
-    hash_auth0 m γ -∗ hash_frag0 k v γ -∗ ⌜m!!k = Some v⌝;
-  hash_frag_frag_agree k v1 v2 γ :
-    hash_frag0 k v1 γ -∗ hash_frag0 k v2 γ -∗ ⌜v1=v2⌝;
-  hash_auth_duplicate_frag m k v γ:
-    m!!k=Some v -> hash_auth0 m γ -∗ hash_frag0 k v γ;
-  hash_auth_insert m k v γ:
-    m!!k=None -> hash_auth0 m γ ==∗ (hash_auth0 (<[k:=v]> m) γ ∗ hash_frag0 k v γ);
-                      
-
-  con_hash_presample0 E (ε:nonnegreal) ns α (ε2 : fin (S val_size) → R) :
+  hash_tape_valid α ns γ:
+    hash_tape0 α ns γ-∗ ⌜Forall (λ x, x<=val_size)%nat ns⌝;
+  hash_tape_exclusive α ns ns' γ:
+    hash_tape0 α ns γ-∗ hash_tape0 α ns' γ-∗ False;
+  hash_tape_auth_exclusive m m' γ:
+    hash_tape_auth0 m γ -∗ hash_tape_auth0 m' γ -∗ False;
+  hash_tape_auth_frag_agree m α ns γ:
+    hash_tape_auth0 m γ  -∗ hash_tape0 α ns γ -∗ ⌜m!!α=Some ns⌝;
+  (* hash_tape_auth_alloc m α γ: *)
+  (*   m!!α=None -> hash_tape_auth0 m γ ==∗ hash_tape_auth0 (<[α:=[]]> m) γ ∗ hash_tape0 α [] γ; *)
+  hash_tape_presample m γ α ns ε ε2 E:
     (∀ x : fin (S val_size), (0 <= ε2 x)%R)->
     (SeriesC (λ n : fin (S val_size), 1 / S val_size * ε2 n) <= ε)%R ->
-    hash_tape0 α ns -∗
-    ↯ ε -∗
-    state_update E E (∃ n,
+    hash_tape_auth0 m γ -∗ hash_tape0 α ns γ -∗ ↯ ε -∗
+    state_update E E (∃ n, 
           ↯ (ε2 n) ∗
-          hash_tape0 α (ns++[fin_to_nat n]) 
-      );
+          hash_tape_auth0 (<[α:=ns++[fin_to_nat n]]>m) γ ∗
+          hash_tape0 α (ns++[fin_to_nat n]) γ); 
+  (* hash_auth_exclusive m m' γ: *)
+  (*   hash_auth0 m γ -∗ hash_auth0 m' γ -∗ False; *)
+  (* hash_auth_frag_agree m k v γ: *)
+  (*   hash_auth0 m γ -∗ hash_frag0 k v γ -∗ ⌜m!!k = Some v⌝; *)
+  (* hash_frag_frag_agree k v1 v2 γ : *)
+  (*   hash_frag0 k v1 γ -∗ hash_frag0 k v2 γ -∗ ⌜v1=v2⌝; *)
+  (* hash_auth_duplicate_frag m k v γ: *)
+  (*   m!!k=Some v -> hash_auth0 m γ -∗ hash_frag0 k v γ; *)
+  (* hash_auth_insert m k v γ: *)
+  (*   m!!k=None -> hash_auth0 m γ ==∗ (hash_auth0 (<[k:=v]> m) γ ∗ hash_frag0 k v γ); *)
+                      
 
-  con_hash_init0 N:
-    {{{ True }}}
+  con_hash_presample0 N f l hm P {HP: ∀ m m', Timeless (P m m')} γ γ_lock Q
+    E  :
+    ↑N ⊆ E ->
+    con_hash_inv0 N f l hm P γ γ_lock -∗
+    (∀ m m', P m m'  -∗
+             hash_tape_auth0 m' γ -∗
+             state_update (E∖↑N) (E∖↑N)
+             (∃ m'', P m m'' ∗ hash_tape_auth0 m'' γ ∗ Q m m' m'')
+    ) -∗
+    state_update E E (
+        ∃ m m' m'', Q m m' m''
+      ); 
+
+  con_hash_init0 N P {HP: ∀ m m', Timeless (P m m')} :
+    {{{ P ∅ ∅ }}}
       init_hash0 #()
-      {{{ (f:val), RET f; ∃ l hm γ1 γ_lock, con_hash_inv0 N f l hm γ1 γ_lock }}};
+      {{{ (f:val), RET f; ∃ l hm γ_tape γ_lock, con_hash_inv0 N f l hm P γ_tape γ_lock }}}; 
 
-  con_hash_alloc_tape0:
-    {{{ True }}}
+  con_hash_alloc_tape0 N f l hm P {HP: ∀ m m', Timeless (P m m')} γ_tape γ_lock Q:
+  {{{ con_hash_inv0 N f l hm P γ_tape γ_lock ∗
+      (∀ m m' α, P m m' -∗ ⌜α∉dom m'⌝ -∗ |={⊤∖↑N}=> P m (<[α:=[]]>m') ∗ Q α)
+  }}}
       allocate_tape0 #()
-      {{{ (α: val), RET α; hash_tape0 α [] }}};
+      {{{ (α: val), RET α; hash_tape0 α [] γ_tape ∗ Q α }}}; 
   
-  con_hash_spec0 N f l hm γ1 γlock α ns (v:nat) P Q:
-  {{{ con_hash_inv0 N f l hm γ1 γlock ∗ hash_tape0 α (ns) ∗
-      ( ∀ m, hash_auth0 m γ1 ={⊤∖↑N}=∗
+  con_hash_spec0 N f l hm P {HP: ∀ m m', Timeless (P m m')} γ_tape γ_lock Q1 Q2 α ns (v:nat):
+  {{{ con_hash_inv0 N f l hm P γ_tape γ_lock ∗ hash_tape0 α (ns) γ_tape∗
+      ( ∀ m m', P m m' -∗ ⌜m'!!α=Some ns⌝ -∗ |={⊤∖↑N}=>
              match m!!v with
-             | Some res => hash_auth0 m γ1 ∗ P res
-             | None => ∃ n ns', ⌜n::ns'=ns⌝ ∗ hash_auth0 (<[v:=n]> m) γ1 ∗ Q
+             | Some res => P m m' ∗ Q1 res
+             | None => ∃ n ns', ⌜n::ns'=ns⌝ ∗ P (<[v:=n]> m) (<[α:=ns']> m') ∗ Q2
              end                                        
       )
   }}}
       f #v α
-      {{{ (res:nat), RET (#res);  (hash_tape0 α (ns) ∗ P res ∨
-                                 ∃ n ns', ⌜n::ns'=ns⌝ ∗ hash_tape0 α ns' ∗ ⌜res=n⌝ ∗ Q 
+      {{{ (res:nat), RET (#res);  (hash_tape0 α (ns) γ_tape ∗ Q1 res ∨
+                                 ∃ n ns', ⌜n::ns'=ns⌝ ∗ hash_tape0 α ns' γ_tape ∗ ⌜res=n⌝ ∗ Q2 
                                 )
       }}};
   (* con_hash_spec_hashed_before0 f l hm γ1 γ2 γlock α ns res (v:nat): *)
@@ -98,44 +118,44 @@ Class con_hash0 `{!conerisGS Σ} (val_size:nat):= Con_Hash0
   (*     }}} *)
 }.
 
-Section test.
-  Context `{conerisGS Σ, !con_hash0 val_size}.
-  Lemma con_hash_spec0' N f l hm γ1 γlock α n ns (v:nat):
-    {{{ con_hash_inv0 N f l hm γ1 γlock ∗ hash_tape0 α (n::ns) }}}
-      f #v α
-      {{{ (res:nat), RET (#res);  hash_frag0 v res γ1 ∗
-                                (hash_tape0 α ns ∗ ⌜res=n⌝ ∨
-                                 hash_tape0 α (n::ns)
-                                )
-      }}}.
-  Proof.
-    iIntros (Φ) "[#Hinv Ht] HΦ".
-    iApply (con_hash_spec0 _ _ _ _ _ _ _ _ _ (λ res, hash_frag0 v res γ1) (hash_frag0 v n γ1) with "[$Hinv $Ht]").
-    - iIntros (m) "Hauth".
-      case_match.
-      + iModIntro.
-        iDestruct (hash_auth_duplicate_frag with "[$]") as "#?"; first done.
-        by iFrame.
-      + iMod (hash_auth_insert with "[$]"); first done.
-        iFrame. iModIntro. by iExists _. 
-    - iNext. iIntros (res) "[[??]|(%&%&%&?&%&?)]"; iApply "HΦ"; iFrame.
-      simplify_eq. iFrame.
-      iLeft. by iFrame.
-  Qed.
+(* Section test. *)
+(*   Context `{conerisGS Σ, !con_hash0 val_size}. *)
+(*   Lemma con_hash_spec0' N f l hm γ1 γlock α n ns (v:nat): *)
+(*     {{{ con_hash_inv0 N f l hm γ1 γlock ∗ hash_tape0 α (n::ns) }}} *)
+(*       f #v α *)
+(*       {{{ (res:nat), RET (#res);  hash_frag0 v res γ1 ∗ *)
+(*                                 (hash_tape0 α ns ∗ ⌜res=n⌝ ∨ *)
+(*                                  hash_tape0 α (n::ns) *)
+(*                                 ) *)
+(*       }}}. *)
+(*   Proof. *)
+(*     iIntros (Φ) "[#Hinv Ht] HΦ". *)
+(*     iApply (con_hash_spec0 _ _ _ _ _ _ _ _ _ (λ res, hash_frag0 v res γ1) (hash_frag0 v n γ1) with "[$Hinv $Ht]"). *)
+(*     - iIntros (m) "Hauth". *)
+(*       case_match. *)
+(*       + iModIntro. *)
+(*         iDestruct (hash_auth_duplicate_frag with "[$]") as "#?"; first done. *)
+(*         by iFrame. *)
+(*       + iMod (hash_auth_insert with "[$]"); first done. *)
+(*         iFrame. iModIntro. by iExists _.  *)
+(*     - iNext. iIntros (res) "[[??]|(%&%&%&?&%&?)]"; iApply "HΦ"; iFrame. *)
+(*       simplify_eq. iFrame. *)
+(*       iLeft. by iFrame. *)
+(*   Qed. *)
 
-  Lemma con_hash_spec_hashed_before N f l hm γ1 γlock α ns res (v:nat):
-    {{{ con_hash_inv0 N f l hm γ1 γlock ∗ hash_tape0 α ns ∗ hash_frag0 v res γ1}}}
-      f #v α
-      {{{ RET (#res);  hash_frag0 v res γ1 ∗
-                       (hash_tape0 α ns)
-      }}}.
-  Proof.
-    iIntros (Φ) "(#Hinv & Ht & #Hfrag) HΦ".
-    iApply (con_hash_spec0 _ _ _ _ _ _ _ _ _ (λ res', ⌜res=res'⌝∗ hash_frag0 v res γ1)%I (False) with "[$Hinv $Ht]").
-    - iIntros. iDestruct (hash_auth_frag_agree with "[$][//]") as "->".
-      iFrame. iModIntro. by iSplit. 
-    - iNext. iIntros (?) "[(?&->&?)|(%&%&%&?&%&%)]"; last done.
-      iApply "HΦ".
-      iFrame.
-  Qed.
-End test.
+(*   Lemma con_hash_spec_hashed_before N f l hm γ1 γlock α ns res (v:nat): *)
+(*     {{{ con_hash_inv0 N f l hm γ1 γlock ∗ hash_tape0 α ns ∗ hash_frag0 v res γ1}}} *)
+(*       f #v α *)
+(*       {{{ RET (#res);  hash_frag0 v res γ1 ∗ *)
+(*                        (hash_tape0 α ns) *)
+(*       }}}. *)
+(*   Proof. *)
+(*     iIntros (Φ) "(#Hinv & Ht & #Hfrag) HΦ". *)
+(*     iApply (con_hash_spec0 _ _ _ _ _ _ _ _ _ (λ res', ⌜res=res'⌝∗ hash_frag0 v res γ1)%I (False) with "[$Hinv $Ht]"). *)
+(*     - iIntros. iDestruct (hash_auth_frag_agree with "[$][//]") as "->". *)
+(*       iFrame. iModIntro. by iSplit.  *)
+(*     - iNext. iIntros (?) "[(?&->&?)|(%&%&%&?&%&%)]"; last done. *)
+(*       iApply "HΦ". *)
+(*       iFrame. *)
+(*   Qed. *)
+(* End test. *)
