theories/coneris/examples/hash/con_hash_interface1.v
@@ -16,76 +16,199 @@ Class con_hash1 `{!conerisGS Σ} (val_size:nat):= Con_Hash1
   
   hash_view_gname:Type;
   hash_set_gname:Type;
+  hash_tape_gname: Type;
   hash_lock_gname:Type;
   
   (** * Predicates *)
-  con_hash_inv1 (f l hm: val) (γ1:hash_view_gname) (γ3: hash_set_gname) (γ_lock:hash_lock_gname): iProp Σ;
+  con_hash_inv1 (N:namespace) (f l hm: val) (P:gmap nat nat -> gmap val (list nat) -> iProp Σ) {HP: ∀ m m', Timeless (P m m')} (γ1:hash_view_gname) (γ2: hash_set_gname) (γ3:hash_tape_gname) (γ_lock:hash_lock_gname): iProp Σ;
   (* concrete_seq_hash {L:seq_hashG Σ} (f:val) (m:gmap nat nat) : iProp Σ;  *)
-  hash_tape1 (α:val) (ns:list nat) (γ3: hash_set_gname): iProp Σ;
-  con_hash_view1 (v res:nat) (γ:hash_view_gname) (γ3 : hash_set_gname): iProp Σ;
-  hash_set1 (s: gset nat) (γ3:hash_set_gname) : iProp Σ; 
+  hash_tape1 (α:val) (ns:list nat) (γ2: hash_set_gname) (γ3:hash_tape_gname): iProp Σ;
+  hash_tape_auth1 (m:gmap val (list nat)) (γ2 :hash_set_gname) (γ3:hash_tape_gname): iProp Σ;
+  hash_auth1 (m:gmap nat nat) (γ:hash_view_gname) (γ2 : hash_set_gname): iProp Σ;
+  hash_frag1 (v res:nat) (γ:hash_view_gname) (γ2 : hash_set_gname): iProp Σ;
+  hash_set1 (s: gset nat) (γ2:hash_set_gname) : iProp Σ;
+  hash_set_frag1 (n:nat) (γ2:hash_set_gname) : iProp Σ;
   
   (** * General properties of the predicates *)
   (* #[global] concrete_seq_hash_timeless {L : seq_hashG Σ} f m :: *)
   (*   Timeless (concrete_seq_hash (L:=L) f m); *)
-  #[global] hash_tape_timeless α ns γ3::
-    Timeless (hash_tape1 α ns γ3 ); 
-  #[global] con_hash_view_timeless v res γ γ3::
-    Timeless (con_hash_view1 v res γ γ3);
-  #[global] hash_set_timeless s γ3 ::
-    Timeless (hash_set1 s γ3);
-  #[global] con_hash_inv_persistent f l hm γ1 γ3 γ_lock ::
-    Persistent (con_hash_inv1 f l hm γ1 γ3 γ_lock);
-  #[global] con_hash_view_persistent v res γ γ3::
-    Persistent (con_hash_view1 v res γ γ3);
-  con_hash_view_frag_frag_agree k v1 v2 γ γ3:
-    con_hash_view1 k v1 γ γ3 -∗ con_hash_view1 k v2 γ γ3-∗ ⌜v1=v2⌝; 
-  con_hash_view_in_hash_set γ1 γ3 s v res:
-    con_hash_view1 v res γ1 γ3 -∗ hash_set1 s γ3 -∗ ⌜res ∈ s⌝ ;
-  hash_tape_in_hash_set α ns γ s:
-    hash_tape1 α ns γ -∗ hash_set1 s γ -∗ ⌜Forall (λ x, x∈s) ns⌝;
-  hash_tape_valid α ns γ3:
-    hash_tape1 α ns γ3-∗ ⌜Forall (λ x, x<=val_size)%nat ns⌝;
+  #[global] hash_tape_timeless α ns γ2 γ3::
+    Timeless (hash_tape1 α ns γ2 γ3);
+  #[global] hash_tape_auth_timeless m γ2 γ3::
+    Timeless (hash_tape_auth1 m γ2 γ3);
+  #[global] hash_auth_timeless m γ γ2::
+    Timeless (hash_auth1 m γ γ2);
+  #[global] hash_frag_timeless v res γ γ2::
+    Timeless (hash_frag1 v res γ γ2);
+  #[global] hash_set_timeless s γ2 ::
+    Timeless (hash_set1 s γ2); 
+  #[global] hash_set_frag_timeless s γ2 ::
+    Timeless (hash_set_frag1 s γ2); 
+  #[global] con_hash_inv_persistent N f l hm γ1 γ2 γ3 P {HP: ∀ m m', Timeless (P m m')} γ_lock ::
+    Persistent (con_hash_inv1 N f l hm P γ1 γ2 γ3 γ_lock); 
+  #[global] hash_frag_persistent v res γ γ2::
+    Persistent (hash_frag1 v res γ γ2);
+  #[global] hash_set_frag_persistent s γ2 ::
+    Persistent (hash_set_frag1 s γ2); 
+  hash_auth_exclusive m m' γ γ2:
+    hash_auth1 m γ γ2 -∗ hash_auth1 m' γ γ2 -∗ False;
+  hash_auth_frag_agree m k v γ γ2:
+    hash_auth1 m γ γ2 -∗ hash_frag1 k v γ γ2 -∗ ⌜m!!k=Some v⌝;
+  hash_auth_duplicate m k v γ γ2:
+    m!!k=Some v -> hash_auth1 m γ γ2 -∗ hash_frag1 k v γ γ2;
+  hash_frag_frag_agree k v1 v2 γ γ2:
+    hash_frag1 k v1 γ γ2 -∗ hash_frag1 k v2 γ γ2-∗ ⌜v1=v2⌝; 
+  hash_frag_in_hash_set γ1 γ2 v res:
+    hash_frag1 v res γ1 γ2 -∗ hash_set_frag1 res γ2 ;
+  hash_tape_in_hash_set α ns γ γ':
+  hash_tape1 α ns γ γ' -∗ [∗ list] n ∈ ns, hash_set_frag1 n γ;
+  hash_set_frag_in_set s n γ:
+  hash_set1 s γ -∗ hash_set_frag1 n γ -∗ ⌜n ∈ s⌝;
+  hash_auth_insert m k v γ1 γ2:
+    m!!k=None -> hash_set_frag1 v γ2 -∗ hash_auth1 m γ1 γ2 ==∗ hash_auth1 (<[k:=v]> m ) γ1 γ2;
+  hash_tape_auth_exclusive m m' γ2 γ3:
+    hash_tape_auth1 m γ2 γ3 -∗ hash_tape_auth1 m' γ2 γ3 -∗ False;
+  hash_tape_auth_frag_agree m α ns γ2 γ3:
+    hash_tape_auth1 m γ2 γ3 -∗ hash_tape1 α ns γ2 γ3 -∗ ⌜m!!α=Some ns⌝;
+  (* hash_tape_auth_insert m α γ2 γ3: *)
+  (*   m!!α=None -> hash_tape_auth1 m γ2 γ3 ==∗ hash_tape_auth1 (<[α:=[]]> m) γ2 γ3 ∗ hash_tape1 α [] γ2 γ3; *)
+  (* hash_tape_auth_frag_update m α ns n γ2 γ3: *)
+  (* hash_set_frag1 n γ2 -∗ hash_tape_auth1 m γ2 γ3 -∗ hash_tape1 α ns γ2 γ3 ==∗ *)
+  (* hash_tape_auth1 (<[α:=ns++[n]]> m) γ2 γ3 ∗ hash_tape1 α (ns ++ [n]) γ2 γ3; *)
+  hash_set_valid s γ:
+    hash_set1 s γ -∗ ⌜∀ n, n∈s -> (n<=val_size)%nat⌝;
+  hash_tape_valid α ns γ2 γ3:
+    hash_tape1 α ns γ2 γ3-∗ ⌜Forall (λ x, x<=val_size)%nat ns⌝; 
+  hash_tape_exclusive α ns ns' γ2 γ3:
+      hash_tape1 α ns γ2 γ3-∗ hash_tape1 α ns' γ2 γ3 -∗ False;
 
-  (** need to update *)
-  con_hash_presample1 γ3 E (ε εI εO:nonnegreal) ns α s :
-    (εI * (size s) + εO * (val_size + 1 - size s) <= ε * (val_size + 1))%R ->
-    hash_tape1 α ns γ3 -∗
-    ↯ ε -∗
-    hash_set1 s γ3 -∗
-    state_update E E (∃ (n:fin (S val_size)),
-          hash_tape1 α (ns++[fin_to_nat n]) γ3 ∗
-          ( (⌜fin_to_nat n ∈ s⌝) ∗ hash_set1 s γ3 ∗ ↯ εI ∨
-            (⌜fin_to_nat n ∉ s⌝) ∗ hash_set1 (s∪{[(fin_to_nat n)]}) γ3 ∗ ↯ εO
-          )
-      );
-
-  con_hash_init1:
-    {{{ True }}}
-      init_hash1 #()
-      {{{ (f:val), RET f; ∃ l hm γ1 γ3 γ_lock, con_hash_inv1 f l hm γ1 γ3 γ_lock ∗
-                                                  hash_set1 ∅ γ3
-      }}};
-
-  con_hash_alloc_tape1 f l hm γ1 γ3 γ_lock:
-    {{{ con_hash_inv1 f l hm γ1 γ3 γ_lock }}}
-      allocate_tape1 #()
-      {{{ (α: val), RET α; hash_tape1 α [] γ3 }}};
   
-  con_hash_spec1 f l hm γ1 γ3 γlock α n ns (v:nat):
-    {{{ con_hash_inv1 f l hm γ1 γ3 γlock ∗ hash_tape1 α (n::ns) γ3 }}}
+  hash_tape_presample m γ γ_set α ns s (ε εI εO:nonnegreal) E:
+    (εI * (size s) + εO * (val_size + 1 - size s) <= ε * (val_size + 1))%R ->
+    hash_tape_auth1 m γ_set γ -∗ hash_tape1 α ns γ_set γ -∗ ↯ ε -∗
+    hash_set1 s γ_set -∗
+    state_update E E (∃ (n:fin(S val_size)), 
+          ( (⌜fin_to_nat n ∈ s⌝) ∗ hash_set1 s γ_set ∗ ↯ εI  ∨
+            (⌜fin_to_nat n ∉ s⌝) ∗ hash_set1 (s∪{[(fin_to_nat n)]}) γ_set ∗ ↯ εO
+          )∗
+          hash_tape_auth1 (<[α:=ns++[fin_to_nat n]]>m) γ_set γ ∗
+          hash_tape1 α (ns++[fin_to_nat n]) γ_set γ
+      ); 
+
+  con_hash_presample1  N f l hm P {HP: ∀ m m', Timeless (P m m')} γ_hv γ_set γ_tape γ_lock Q
+    E  :
+    ↑N ⊆ E ->
+    con_hash_inv1 N f l hm P γ_hv γ_set γ_tape γ_lock -∗
+    (∀ m m', P m m'  -∗
+             hash_tape_auth1 m' γ_set γ_tape -∗
+             state_update (E∖↑N) (E∖↑N)
+             (∃ m'', P m m'' ∗ hash_tape_auth1 m'' γ_set γ_tape ∗ Q m m' m'')
+    ) -∗
+    state_update E E (
+        ∃ m m' m'', Q m m' m''
+      ) ;
+
+  con_hash_init1 N P {HP: ∀ m m', Timeless (P m m')}:
+    {{{ P ∅ ∅ }}}
+      init_hash1 #()
+      {{{ (f:val), RET f; ∃ l hm γ1 γ2 γ3 γ_lock, con_hash_inv1 N f l hm P γ1 γ2 γ3 γ_lock ∗
+                                                  hash_set1 ∅ γ2
+      }}}; 
+
+  con_hash_alloc_tape1 N f l hm P {HP: ∀ m m', Timeless (P m m')} γ1 γ2 γ3 γ_lock Q:
+  {{{ con_hash_inv1 N f l hm P γ1 γ2 γ3 γ_lock ∗
+      (∀ m m' α, P m m' -∗ ⌜α∉dom m'⌝ -∗ |={⊤∖↑N}=> P m (<[α:=[]]>m') ∗ Q α)
+  }}}
+      allocate_tape1 #()
+      {{{ (α: val), RET α; hash_tape1 α [] γ2 γ3 ∗ Q α }}}; 
+
+  con_hash_spec1 N f l hm P {HP: ∀ m m', Timeless (P m m')} γ1 γ2 γ3 γ_lock Q1 Q2 α ns (v:nat):
+  {{{ con_hash_inv1 N f l hm P γ1 γ2 γ3 γ_lock ∗ hash_tape1 α (ns) γ2 γ3∗
+      ( ∀ m m', P m m' ∗ hash_auth1 m γ1 γ2 -∗ ⌜m'!!α=Some ns⌝ -∗ |={⊤∖↑N}=>
+             match m!!v with
+             | Some res => P m m' ∗ hash_auth1 m γ1 γ2 ∗ Q1 res
+             | None => ∃ n ns', ⌜n::ns'=ns⌝ ∗ P (<[v:=n]> m) (<[α:=ns']> m')∗ hash_auth1 (<[v:=n]> m) γ1 γ2  ∗ Q2
+             end                                        
+      )
+  }}}
       f #v α
-      {{{ (res:nat), RET (#res);  con_hash_view1 v res γ1 γ3 ∗
-                                (hash_tape1 α ns γ3 ∗ ⌜res=n⌝ ∨
-                                 hash_tape1 α (n::ns) γ3
+      {{{ (res:nat), RET (#res);  (hash_tape1 α (ns) γ2 γ3 ∗ Q1 res ∨
+                                 ∃ n ns', ⌜n::ns'=ns⌝ ∗ hash_tape1 α ns' γ2 γ3 ∗ ⌜res=n⌝ ∗ Q2 
                                 )
       }}};
-  
-  con_hash_spec_hashed_before1 f l hm γ1 γ3 γlock α ns res (v:nat):
-    {{{ con_hash_inv1 f l hm γ1 γ3 γlock ∗ hash_tape1 α ns γ3 ∗ con_hash_view1 v res γ1 γ3 }}}
-      f #v α
-      {{{ RET (#res);  con_hash_view1 v res γ1 γ3 ∗
-                       (hash_tape1 α ns γ3 )
-      }}}
 }.
 
+Section test.
+  Context `{conerisGS Σ, !con_hash1 val_size}.
+
+  Lemma con_hash_presample_test N f l hm γ1 γ2 γ3 γlock  E (ε εI εO:nonnegreal) ns α s :
+    ↑N⊆E ->
+    (εI * (size s) + εO * (val_size + 1 - size s) <= ε * (val_size + 1))%R ->
+    con_hash_inv1 N f l hm (λ _ _, True) γ1 γ2 γ3 γlock -∗
+    hash_tape1 α ns γ2 γ3 -∗
+    ↯ ε -∗
+    hash_set1 s γ2 -∗
+    state_update E E (∃ (n:fin (S val_size)),
+          hash_tape1 α (ns++[fin_to_nat n]) γ2 γ3 ∗
+          ( (⌜fin_to_nat n ∈ s⌝) ∗ hash_set1 s γ2 ∗ ↯ εI ∨
+            (⌜fin_to_nat n ∉ s⌝) ∗ hash_set1 (s∪{[(fin_to_nat n)]}) γ2 ∗ ↯ εO
+          )
+      ).
+  Proof.
+    iIntros (Hsubset Hineq) "#Hinv Ht Herr Hs".
+    iMod (con_hash_presample1 _ _ _ _ _ _ _ _ _
+            (λ m m' m'', (∃ n : fin (S val_size), hash_tape1 α (ns ++ [fin_to_nat n]) γ2 γ3 ∗
+                                                  (⌜fin_to_nat n ∈ s⌝ ∗ hash_set1 s γ2 ∗ ↯ εI ∨ ⌜fin_to_nat n ∉ s⌝ ∗ hash_set1 (s ∪ {[fin_to_nat n]}) γ2 ∗ ↯ εO)))%I with "[//][-]") as "Hcont"; first done.
+    - iIntros (_ ?) "_ Hauth".
+      iMod (hash_tape_presample with "[$][$][$][$]") as "(%&?&$&$)"; first done.
+      by iFrame.
+    - iDestruct "Hcont" as "(%&%&%&%&$&[(%&?&?)|(%&?&?)])"; iModIntro; [iLeft|iRight]; by iFrame.
+  Qed.
+  
+    
+  Lemma con_hash_spec_test1 N f l hm γ1 γ2 γ3 γlock α n ns (v:nat):
+    {{{ con_hash_inv1 N f l hm (λ _ _, True) γ1 γ2 γ3 γlock ∗ hash_tape1 α (n::ns) γ2 γ3 }}}
+      f #v α
+      {{{ (res:nat), RET (#res);  hash_frag1 v res γ1 γ2 ∗
+                                (hash_tape1 α ns γ2 γ3 ∗ ⌜res=n⌝ ∨
+                                 hash_tape1 α (n::ns) γ2 γ3
+                                )
+      }}}.
+  Proof.
+    iIntros (Φ) "[#Hinv Ht] HΦ".
+    iDestruct (hash_tape_in_hash_set with "[$]") as "#Hfrag".
+    iApply (con_hash_spec1 _ _ _ _ _ _ _ _ _ (λ res, hash_frag1 v res γ1 γ2) (hash_frag1 v n γ1 γ2) with "[$Hinv $Ht]").
+    - iIntros (??) "[_ Hauth] %".
+      case_match.
+      + by iDestruct (hash_auth_duplicate with "[$]") as "#$"; first done.
+      + iMod (hash_auth_insert with "[][$]") as "H"; first done; last first.
+        * iDestruct (hash_auth_duplicate with "[$]") as "#$"; first by rewrite lookup_insert.
+          iFrame. iModIntro. by iExists _.
+        * rewrite big_sepL_cons. iDestruct "Hfrag" as "[$ ?]".        
+    - iNext. iIntros (res) "[[??]|(%&%&%&?&%&H)]".
+      + iApply "HΦ". iFrame.
+      + iApply "HΦ". simplify_eq. iFrame "H". iLeft. by iFrame.
+  Qed.
+
+  Lemma con_hash_spec_hashed_before1 N f l hm γ1 γ2 γ3 γlock α ns res (v:nat):
+    {{{ con_hash_inv1 N f l hm (λ _ _, True) γ1 γ2 γ3 γlock ∗ hash_tape1 α ns γ2 γ3 ∗ hash_frag1 v res γ1 γ2 }}}
+      f #v α
+      {{{ RET (#res);  hash_frag1 v res γ1 γ2 ∗
+                       (hash_tape1 α ns γ2 γ3 )
+      }}}.
+  Proof. 
+    iIntros (Φ) "(#Hinv & Ht & #Hf) HΦ".
+    iDestruct (hash_tape_in_hash_set with "[$]") as "#Hfrag".
+    iApply (con_hash_spec1 _ _ _ _ _ _ _ _ _ (λ res' , ⌜res=res'⌝ ∗ hash_frag1 v res γ1 γ2)%I (False) with "[$Hinv $Ht]").
+    - iIntros (??) "[_ Hauth] %".
+      case_match.
+      + iDestruct (hash_auth_frag_agree with "[$][$]") as "%".
+        simplify_eq. iDestruct (hash_auth_duplicate with "[$]") as "#$"; first done. by iFrame.
+      + iDestruct (hash_auth_frag_agree with "[$][$]") as "%".
+        simplify_eq.
+    - iNext. iIntros (res') "[[?[->?]]|(%&%&%&?&?&%)]".
+      + iApply "HΦ". iFrame.
+      + done.
+  Qed.
+  
+End test.
